saving state of the work

src_arrays/LambdaTotalTriple_credits_perm.v
@@ -1,5 +1,6 @@
 Require List.
 Import List.ListNotations.
+Require Vector.
 Require Import String.
 Require Import ZArith.
 
@@ -42,3 +43,145 @@ Definition triple_fun {V : Set}
   (v : Value V)
   (P Q : Value V -> StateAssertion V) : Prop :=
   forall v' : Value V, triple (v <* v') (P v') Q.
+
+(*Fixpoint n_ary_StateAssertion (n : nat) V :=
+  match n with
+  | 0 => StateAssertion V
+  | S n' => Value V -> n_ary_StateAssertion n' V
+  end.
+
+Fixpoint n_ary_forall*)
+
+Fixpoint n_ary_app {V : Set} (e : Expr V) (es : list (Expr V)) : Expr V :=
+  match es with
+  | [] => e
+  | (e'::es') => n_ary_app (e <* e') es'
+  end%list.
+
+(*
+Definition triple_fun_n_ary {V : Set} n
+  (v : Value V)
+  (P : list (Value V) -> StateAssertion V)
+  (Q : Value V -> StateAssertion V) : Prop :=
+  forall vs : list (Value V),
+    List.length vs = n -> triple (n_ary_app v (List.map Val vs)) (P vs) Q.
+
+Fixpoint triple_list {V : Set}
+  (es : list (Expr V))
+  (P : StateAssertion V)
+  (Q : list (Value V) -> StateAssertion V) : Prop :=
+  match es with
+  | [] => P ->> Q []
+  | (e::es') =>
+    exists Q', triple e P Q' /\
+      forall v, triple_list es' (Q' v) (fun vs => Q (v::vs))
+  end%list.
+
+(*Fixpoint triple_list_decreasing {V : Set}
+  (es : list (Expr V))
+  (P : StateAssertion V)
+  (Q : list (Value V) -> StateAssertion V) : Prop :=
+  match es with
+  | [] => P ->> Q []
+  | (e::es') =>
+    exists P', P ->> $1 <*> P' /\
+    exists Q', triple e P' Q' /\
+      forall v, triple_list_decreasing es' (Q' v) (fun vs => Q (v::vs))
+  end%list.*)
+
+Fixpoint n_ary_app_inv {V : Set} (e : Expr V) (es : list (Expr V)) : Expr V :=
+  match es with
+  | [] => e
+  | (e'::es') => n_ary_app_inv e es' <* e'
+  end%list.
+
+Definition triple_fun_n_ary_inv {V : Set} n
+  (v : Value V)
+  (P : list (Value V) -> StateAssertion V)
+  (Q : Value V -> StateAssertion V) : Prop :=
+  forall vs : list (Value V),
+    List.length vs = n -> triple (n_ary_app_inv v (List.map Val vs)) (P vs) Q.
+
+Fixpoint triple_list_inv {V : Set}
+  (es : list (Expr V))
+  (P : StateAssertion V)
+  (Q : list (Value V) -> StateAssertion V) : Prop :=
+  match es with
+  | [] => P ->> Q []
+  | (e::es') =>
+    exists Q', triple_list_inv es' P Q' /\
+      forall vs, triple e (Q' vs) (fun v => Q (v::vs))
+  end%list.
+*)
+
+Fixpoint n_ary_fun_type (n : nat) (A B : Type) : Type :=
+  match n with
+  | 0 => B
+  | S n' => A -> n_ary_fun_type n' A B
+  end.
+
+Fixpoint n_ary_fun_app {A B : Type} (xs : list A) :
+  n_ary_fun_type (List.length xs) A B -> B :=
+  match xs with
+  | [] => fun f => f
+  | (x::xs') => fun f => n_ary_fun_app xs' (f x)
+  end%list.
+
+Fixpoint n_ary_forall n [A : Type] : n_ary_fun_type n A Type -> Type :=
+  match n with
+  | 0 => fun B => B
+  | S n' => fun B => forall x : A, n_ary_forall n' (B x)
+  end.
+
+Fixpoint to_n_ary_fun {A B} (n : nat) :
+  (Vector.t A n -> B) -> n_ary_fun_type n A B :=
+  match n return (Vector.t A n -> B) -> n_ary_fun_type n A B with
+  | 0 => fun f => f (Vector.nil _)
+  | S n' => fun f x => to_n_ary_fun n' (fun xs => f (Vector.cons _ x _ xs))
+  end.
+
+Fixpoint to_n_ary_fun' {A B} (n : nat) (f : (list A -> B)) :
+  n_ary_fun_type n A B :=
+  match n return n_ary_fun_type n A B with
+  | 0 => f nil
+  | S n' => fun x => to_n_ary_fun' n' (fun xs => f (cons x xs))
+  end.
+
+(* a triple for n+1-argument function *)
+Fixpoint triple_fun_n_ary n {V : Set}
+  (v : Value V) :
+  (Value V -> n_ary_fun_type n (Value V) (StateAssertion V)) ->
+  (Value V -> Value V -> n_ary_fun_type n (Value V) (StateAssertion V)) ->
+    Prop :=
+  match n with
+  | 0 => fun P Q => forall x, triple_fun v (fun v => <[v = x]> <*> P x) (Q x)
+  | S n' => fun P Q => forall x,
+    triple_fun v
+    (fun v => <[v = x]>)
+    (fun v => <[
+      triple_fun_n_ary n' v (P x) (Q x)
+    ]>)
+  end.
+
+Fixpoint triple_list {V : Set}
+  (es : list (Expr V))
+  (P : StateAssertion V) :
+  n_ary_fun_type (List.length es) (Value V) (StateAssertion V) ->
+    Prop :=
+  match es return n_ary_fun_type (List.length es) (Value V) (StateAssertion V) -> Prop with
+  | [] => fun Q => P ->> Q
+  | (e::es') => fun Q =>
+    exists Q', triple e P Q' /\
+      forall v, triple_list es' (Q' v) (Q v)
+  end%list.
+
+(*Eval simpl in triple_fun_n_ary 2.*)
+
+(*Fixpoint triple_fun_n_ary n {V : Set}
+  (v : Value V)
+  (P : n_ary_fun_type n (Value V) (StateAssertion V))
+  (Q : Value V -> StateAssertion V) : Prop :=
+  n_ary_forall n (to_n_ary_fun n (fun xs =>
+    match xs with
+    | Vector.nil _ =>
+    end))*)
